{
 "cells": [
  {
   "cell_type": "markdown",
   "metadata": {},
   "source": [
    "<span style=\"font-size: 14pt\">EREVAN, May-June 2017</span>\n",
    "\n",
    "<span style=\"font-size: 16pt\"> Seminar #2: Exponential smoothing models\n",
    "\n",
    "<span style=\"color:blue; font-size: 12pt\">Alexey Romanenko </span>,\n",
    "<span style=\"color:blue; font-size: 12pt; font-family: 'Verdana'\">alexromsput@gmail.com</span>\n",
    "\n",
    "\n",
    "<h1 align=\"center\"> Home Work 1 </h1>\n",
    "\n",
    "## Answer questions\n",
    "\n",
    "1) ** How do adaptive properties of SES change when smoothing parametr $\\alpha$ converges to 1?**\n",
    "\n",
    "<Answer>\n",
    "\n",
    "2) ** What will be the optimal value of smoothing parameter of trend $\\beta$ in Hold model for 1) time series with slowly  changing trend; 2) stochastic changing trend (look <a href=\"http://stochastictrend.blogspot.am/\">here </a>)? **\n",
    "\n",
    "<Answer>\n",
    "\n",
    "3) **Proof the equivalency of correction error form and smoothing form for unobserved component of TS in  Thei-Wage model (period of seasonality equals $p$):**\n",
    "\n",
    "  $$l_t = \\alpha (y_t - s_{t-p}) + (1-\\alpha) (l_{t-1} + b_{t-1} )=l_{t-1} + b_{t-1} + \\alpha e_t;$$\n",
    "  $$ b_t = \\beta (l_{t} - l_{t-1} ) + (1-\\beta) b_{t-1} = b_{t-1} + \\alpha\\beta e_t;$$\n",
    "  $$ s_t = \\gamma (y_t-l_t) + (1-\\gamma) s_{t-p} = s_{t-p} + \\gamma(1-\\alpha)e_t.$$\n",
    "\n",
    "\n",
    "4) **Find the correction error form for unobserved component of TS in ES with additive damped trend:**\n",
    "\n",
    "$$\\hat{y}_{t+d|t} = l_t + \\left(\\phi + \\phi^2 + \\dots + \\phi^{d}\\right) b_t.$$\n",
    "\n",
    "**Unobserved components are (in smoothing form): **\n",
    "\n",
    "$$ l_{t}       = \\alpha y_t + \\left(1-\\alpha\\right) \\left(l_{t-1} +\\phi b_{t-1}\\right),$$\n",
    "$$ b_t         = \\beta \\left(l_t - l_{t-1}\\right) + \\left(1-\\beta\\right)\\phi b_{t-1}.$$"
   ]
  },
  {
   "cell_type": "markdown",
   "metadata": {},
   "source": [
    "## Answers\n"
   ]
  },
  {
   "cell_type": "markdown",
   "metadata": {},
   "source": [
    "1) When $\\alpha$ converges to 1 graph of predicted values becomes very similar to graph of true values, but with some shift.\n",
    "\n",
    "2) For TS with slowly changing trend we need to choose small $\\beta$ convergeing to 0, and for TS with stochastic changing trend we need to choose big $\\beta$.\n",
    "\n",
    "3)\n",
    "\n",
    "1.$$l_t = \\alpha (y_t - s_{t-p}) + (1-\\alpha) (l_{t-1} + b_{t-1} )=l_{t-1} + b_{t-1} + \\alpha e_t$$\n",
    "Proof \n",
    "$$l_t = \\alpha (y_t - s_{t-p}) + (1-\\alpha) (l_{t-1} + b_{t-1} )= \\alpha (y_t - l_{t-1} - s_{t-p} - b_{t-1}) + l_{t-1} + b_{t-1}$$\n",
    "$$l_{t-1} - s_{t-p} - b_{t-1} = \\hat{y_t}$$\n",
    "$$y_t - l_{t-1} - s_{t-p} - b_{t-1} = y_t - \\hat{y_t} = e_t$$\n",
    "So we get\n",
    "$$l_t = \\alpha (y_t - s_{t-p}) + (1-\\alpha) (l_{t-1} + b_{t-1} ) = l_{t-1} + b_{t-1} + \\alpha e_t$$\n",
    "\n",
    "2.\n",
    "$$ b_t = \\beta (l_{t} - l_{t-1} ) + (1-\\beta) b_{t-1} = b_{t-1} + \\alpha\\beta e_t$$\n",
    "Proof\n",
    "$$ b_t = \\beta (l_{t} - l_{t-1} ) + (1-\\beta) b_{t-1} = \\beta (l_t - l_{t-1} - b_{t-1}) + b_{t-1} = b_{t-1} + \\beta \\alpha e_t$$ (as $l_t - l_{t-1} - b_{t-1} = \\alpha e_t$ from 3.1)\n",
    "\n",
    "3.\n",
    "$$ s_t = \\gamma (y_t-l_t) + (1-\\gamma) s_{t-p} = s_{t-p} + \\gamma(1-\\alpha)e_t$$\n",
    "Proof\n",
    "$$ s_t = \\gamma (y_t-l_t) + (1-\\gamma) s_{t-p} = \\gamma (y_t - l_t - s_{t-p}) + s_{t-p} = s_{t-p} + \\gamma (y_t - l_t - s_{t-p} - l_{t-1} - b_{t-1} + l_{t-1} + b_{t-1}) = s_{t-p} + \\gamma (e_t -\\alpha e_t) = s_{t-p} + \\gamma (1 - \\alpha)e_t$$\n",
    "as $y_t - s_{t-p} - l_{t-1} - b_{t-1} = e_t$ and $l_{t-1} + b_{t-1} - l_t = \\alpha e_t$\n",
    "\n",
    "4)\n",
    "$$\\hat{y}_{t+d|t} = l_t + (\\phi + \\phi^2 + \\dots + \\phi^{d}) b_t$$\n",
    "When $d=1$ we have \n",
    "$$\\hat{y}_{t+1|t} = l_t + \\phi b_t$$\n",
    "$$e_t = y_{t} - \\hat{y_t} = y_{t} - l_{t-1} - \\phi b_{t-1}$$\n",
    "\n",
    "$$ l_{t}       = \\alpha y_t + \\left(1-\\alpha\\right) \\left(l_{t-1} +\\phi b_{t-1}\\right) = \\alpha (y_t - l_{t-1} - \\phi b_{t-1}) + l_{t-1} + \\phi b_{t-1} = \\alpha e_t + l_{t-1} + \\phi b_{t-1}$$\n",
    "\n",
    "$$ b_t         = \\beta \\left(l_t - l_{t-1}\\right) + \\left(1-\\beta\\right)\\phi b_{t-1} = \\beta (\\alpha e_t + \\phi b_{t-1}) + (1-\\beta) \\phi b_{t-1} = \\beta \\alpha e_t + \\phi b_{t-1}$$"
   ]
  }
 ],
 "metadata": {
  "anaconda-cloud": {},
  "kernelspec": {
   "display_name": "Python 3",
   "language": "python",
   "name": "python3"
  },
  "language_info": {
   "codemirror_mode": {
    "name": "ipython",
    "version": 3
   },
   "file_extension": ".py",
   "mimetype": "text/x-python",
   "name": "python",
   "nbconvert_exporter": "python",
   "pygments_lexer": "ipython3",
   "version": "3.6.0"
  }
 },
 "nbformat": 4,
 "nbformat_minor": 1
}
